\documentclass{article}
\usepackage{graphicx} % Required for inserting images
\usepackage[utf8]{inputenc}
\usepackage{amsmath}
\usepackage{graphicx}
\usepackage{tikz}
\usepackage{array}
\usepackage{amssymb}
\newcommand*{\twoheadrightarrowtail}{\mathrel{\rightarrowtail\kern-1.9ex\twoheadrightarrow}}
% Alternative which doesn't look as good using the normal size, but might work better with smaller sizes too:
%\newcommand*{\twoheadrightarrowtail}{\mathrel{\rlap{$\rightarrowtail$}\twoheadrightarrow}}
\usepackage{amssymb}
\usepackage{amsthm}
\usepackage{multirow}
\usepackage{verbatim}
\usepackage{dcolumn}
\newcolumntype{2}{D{.}{}{2.0}}

\title{MATH 265 HW3}
\author{Hanzhang Yin}
\date{Sep/12/2024}

\begin{document}

\maketitle

\section*{Question 1}
\begin{proof}
    proof by contradiction: suppose $a < b$.
    \\
    By assumption, we have $a \geq b - \epsilon$, for all $\epsilon > 0$.
    \\
    define $d = b - a$. Since $a < b$, by definition, $d = b - a \in \mathbb{P} > 0$.
    \\
    Now we pick $\epsilon = \frac{d}{2}$. Since $d > 0$, $\epsilon = \frac{d}{2} > 0$.
    \\
    We know that:
    \[ a \geq b - \epsilon \]
    Sub $\epsilon = \frac{d}{2}$ in, we get:
    \[ a \geq b - \frac{d}{2} \]
    Rewrite the expression in terms of $a$ and $b$ (Note: $d = b - a$):
    \[ a \geq b - \frac{b - a}{2} \Rightarrow a \geq \frac{2b - (b - a)}{2} = \frac{b + a}{2} \]
    Multiply both side by 2 (using A2 and M1), we get:
    \[ 2a \geq b + a \]
    Then, use the A4, subtract $a$ from both sides:
    \[ 2a - a \geq b + a - a \]
    Then, use A1 and A3, we can get:
    \[ a \geq b + (a - a) \Rightarrow a \geq b + 0 \rightarrow a \geq b \]
    Hence we derived a contradiction. Using the field axioms, the given assumption implies $a \geq b$.
\end{proof}

\newpage

\section*{Question 2}
\begin{proof}
    Recall the hint that:
    \[ a^2 - b^2 = (a + b)(a - b) \]
    Sub $b = -a$ into the identity, we can get:
    \[ a^2 - (-a^2) = (a + (-a))(a - (-a)) \]
    Using the axoim of additive inverses (A4): $a + (-a) = 0$.
    \[ \Rightarrow a^2 - (-a^2) = (0)(a - (-a)) \]
    By the Theorem of we know that $a \cdot 0 = 0$ for any $x \in \mathbb{R}$. Thus we have,
    \[ \Rightarrow a^2 - (-a^2) = 0 \Rightarrow a^2  = (-a^2) \]
\end{proof}

\newpage

\section*{Question 3}
\begin{proof}
    First, we want to prove:
    \[ \left( \frac{1}{2} (a + b) \right)^2 \leq \frac{1}{2} (a^2 + b^2) \]
    for all $a,b \in \mathbb{R}$.
    \\
    First using axiom D (distributive property) twice, we can expand LHS:
    \[ \left( \frac{1}{2} (a + b) \right)^2 = \frac{1}{4}(a + b)^2 = \frac{1}{4}(a^2 + 2ab + b^2) \]
    \\
    Now we reform the inequality and WTS that:
    \[ \frac{1}{4}(a^2 + 2ab + b^2) \leq \frac{1}{2} (a^2 + b^2) \]
    Multiply both sides by 4, then use M2, we can get:
    \[ (\frac{1}{4} \cdot 4) \cdot (a^2 + 2ab + b^2) \leq (\frac{1}{4} \cdot \frac{1}{2}) \cdot (a^2 + b^2) \Rightarrow a^2 + 2ab + b^2 \leq 2(a^2 + b^2) \]
    Now we can rearrange terms using A1, A2, and D axiom:
    \[ a^2 + 2ab + b^2 \leq 2a^2 + 2b^2 \Rightarrow a^2 + 2ab + b^2 - 2a^2 - 2b^2 \leq 0 \]
    This simplifies to:
    \[ \Rightarrow -a^2 + 2ab - b^2 \leq 0 \]
    By D axiom again, we can factor out the (-1) as:
    \[ \Rightarrow (-1)(a^2 - 2ab + b^2) \leq 0 \]
    We know that \( a^2 - 2ab + b^2 = (a - b)^2 \), hence:
    \[ \Rightarrow (-1)(a - b)^2 \leq 0 \]
    Therefore, the inequality always holds for $a, b \in \mathbb{R}$.
    \\
    Then we want to show this equality holds iff $a = b$.
    Noting that since $(a - b)^2 \geq 0$, for any $a,b \in \mathbb{R}$, by A4, its additive inverse $(-1)(a - b)^2 \leq 0$ must also hold. Since we have simplified \(\left( \frac{1}{2} (a + b) \right)^2 \leq \frac{1}{2} (a^2 + b^2) \) to \( (-1)(a - b)^2 \leq 0 \). Hence,
    \[ (a - b)^2 = 0 \Leftrightarrow a - b = 0 \Leftrightarrow  a = b \]
    Therefore, the given inequality holds if and only if for $a = b$.
\end{proof}

\end{document}
